PhysLean/StringTheory/FTheory/SU5U1/Quanta/FromParts.lean
@@ -17,217 +17,10 @@ the allowed `FiveQuanta` or `TenQuanta` which can be formed from them.
 
 We do this only in the very restrictive case when:
 - `fluxes` has no exotics and has no zero fluxes
-- `charges` has length less than or equal to `3` and lives in `allowedBarFiveCharges` or
+- `charges` lives in `allowedBarFiveCharges` or
   `allowedBarTenCharges` for a given `CodimensionOneConfig`.
 
 -/
-
-/-!
-
-## Auxiliary Results
-
-Computable permutations of lists of length at most 3.
-
--/
-
-/-- For a list `l` of length less then three `l.lowPermutations` is the
-  list of permutations of `l`. If the length of `l` is greater then three
-  then this returns `[]`. This is defined so one can use `decide` with such permutations. -/
-def _root_.List.lowPermutations : (l : List (ℤ × ℤ)) → List (List (ℤ × ℤ))
-  | [] => [[]]
-  | x :: [] => [[x]]
-  | x1 :: x2 :: [] => if x1 = x2 then [[x1, x2]] else
-    [[x1, x2], [x2, x1]]
-  | x1 :: x2 :: x3 :: [] =>
-    if x1 = x2 ∧ x2 = x3 then
-      [[x1, x2, x3]]
-    else if x1 = x2 then
-      [[x1, x2, x3], [x1, x3, x2], [x3, x1, x2]]
-    else if x2 = x3 then
-      [[x1, x2, x3], [x2, x1, x3], [x2, x3, x1]]
-    else if x1 = x3 then
-      [[x1, x2, x3], [x2, x1, x3], [x1, x3, x2]]
-    else
-      [[x1, x2, x3], [x1, x3, x2], [x2, x1, x3], [x2, x3, x1], [x3, x1, x2], [x3, x2, x1]]
-  | _ :: _ :: _ :: _ => []
-
-lemma _root_.List.lowPermutations_perm_mem_of_length_le_three :
-    (l l1 : List (ℤ × ℤ)) → (h : l.Perm l1) → (hl : l.length ≤ 3) → l1 ∈ l.lowPermutations
-  | [], l1, h, hl => by
-    simpa [List.lowPermutations] using h
-  | x :: [], l1, h, hl => by
-    simpa [List.lowPermutations] using h.symm
-  | x1 :: x2 :: [], l, h, hl => by
-    simp [List.lowPermutations]
-    have hl : l.length = 2 := by
-      rw [← List.Perm.length_eq h]
-      simp
-    rw [List.length_eq_two] at hl
-    obtain ⟨y1, y2, rfl⟩ := hl
-    simp [List.cons_perm_iff_perm_erase] at h
-    by_cases h1 : x1 = y1
-    · subst h1
-      simp at h
-      obtain ⟨h2', h3'⟩ := h
-      subst h2'
-      split
-      · simp
-      · simp
-    · have h1 : x1 = y2 := by
-        simp [h1] at h
-        exact h.1
-      subst h1
-      simp at h
-      rw [List.erase_cons] at h
-      have hn : y1 ≠ x1 := by exact fun a => h1 (id (Eq.symm a))
-      simp [hn] at h
-      obtain ⟨h2', h3'⟩ := h
-      subst h2'
-      split <;> simp_all
-  | x1 :: x2 :: x3 :: [], l1, h, hl => by
-    simp [List.lowPermutations]
-    have hl : l1.length = 3 := by
-      rw [← List.Perm.length_eq h]
-      simp
-    rw [List.length_eq_three] at hl
-    obtain ⟨y1, y2, y3, rfl⟩ := hl
-    simp [List.cons_perm_iff_perm_erase] at h
-    have h1 := h.1
-    by_cases h1 : x1 = y1
-    · subst h1
-      by_cases h2 : x2 = y2
-      · subst h2
-        simp at h
-        have h3 := h.1
-        subst h3
-        split_ifs
-          <;> simp
-      · have h2 : x2 = y3 := by
-          simp [h2] at h
-          exact h.1
-        have h2n : y2 ≠ x2 := by
-          (expose_names; exact fun a => h2_1 (id (Eq.symm a)))
-        subst h2
-        simp at h
-        simp [List.erase_cons, h2n] at h
-        have h3 := h.1
-        subst h3
-        split_ifs <;> simp_all
-    · have h1n : y1 ≠ x1 := by
-        (expose_names; exact fun a => h1 (id (Eq.symm a)))
-      simp [h1n] at h
-      by_cases h1 : x1 = y2
-      · simp [h1] at h
-        by_cases h2 : x2 = y1
-        · simp [h2] at h
-          have h3 := h.1
-          subst h3
-          split_ifs <;> simp_all
-        · have h2 : x2 = y3 := by
-            simp [h2] at h
-            exact h.1
-          have h2n : y1 ≠ x2 := by
-            (expose_names; exact fun a => h2_1 (id (Eq.symm a)))
-          subst h2
-          simp [List.erase_cons, h2n] at h
-          have h3 := h.1
-          subst h3
-          split_ifs <;> simp_all
-      · simp_all
-        expose_names
-        have h2n : y2 ≠ x1 := by
-          exact Ne.symm (Lean.Grind.ne_of_ne_of_eq_left h1_1 h1)
-        subst h1_1 -- x1 = y3
-        by_cases h2 : x2 = y1
-        · subst h2
-          simp [List.erase_cons, h2n] at h
-          have h3 := h.1
-          subst h3
-          split_ifs <;> simp_all
-        · have h3n : y1 ≠ x2 := by
-            exact fun a => h2 (id (Eq.symm a))
-          have h2 : x2 = y2 := by
-            simp [List.erase_cons, h3n, h2n, h1n] at h
-            exact h.2.2.2.symm
-          have h3 : x3 = y1 := by
-            simp [List.erase_cons, h3n, h2n, h1n] at h
-            exact h.2.2.1.symm
-          subst h2 h3
-          split_ifs <;> simp_all
-
-lemma _root_.List.perm_of_mem_lowPermutations_of_length_le_three :
-    (l l1 : List (ℤ × ℤ)) → (h : l1 ∈ l.lowPermutations) → (hl : l.length ≤ 3) → l1.Perm l
-  | [], l1, h, hl => by
-    simpa [List.lowPermutations] using h
-  | x :: [], l1, h, hl => by
-    simp [List.lowPermutations] at h
-    subst h
-    simp
-  | x1 :: x2 :: [], l1, h, hl => by
-    simp [List.lowPermutations] at h
-    split_ifs at h
-    · simp_all
-    · simp_all
-      rcases h with rfl | rfl
-      · simp
-      · exact List.Perm.swap x1 x2 []
-  | x1 :: x2 :: x3 :: [], l1, h, hl => by
-    simp [List.lowPermutations] at h
-    split_ifs at h
-    · simp_all
-    · simp_all
-      rcases h with rfl | rfl | rfl | rfl | rfl | rfl
-      · simp
-      · simp
-        exact List.Perm.swap x2 x3 []
-      · trans [x2, x3, x2]
-        · exact List.Perm.swap x2 x3 [x2]
-        · simp
-          exact List.Perm.swap x2 x3 []
-    · simp_all
-      rcases h with rfl | rfl | rfl | rfl | rfl | rfl
-      · simp
-      · exact List.Perm.swap x1 x3 [x3]
-      · trans [x3, x1, x3]
-        · simp
-          exact List.Perm.swap x1 x3 []
-        · exact List.Perm.swap x1 x3 [x3]
-    · simp_all
-      rcases h with rfl | rfl | rfl | rfl | rfl | rfl
-      · simp
-      · exact List.Perm.swap x3 x2 [x3]
-      · trans [x3, x2, x3]
-        · simp
-          exact List.Perm.swap x2 x3 []
-        · exact List.perm_iff_count.mpr (congrFun rfl)
-    · simp_all
-      rcases h with rfl | rfl | rfl | rfl | rfl | rfl
-      any_goals simp
-      · exact List.Perm.swap x2 x3 []
-      · exact List.Perm.swap x1 x2 [x3]
-      · trans [x2, x1, x3]
-        · simp
-          exact List.Perm.swap x1 x3 []
-        · exact List.Perm.swap x1 x2 [x3]
-      · trans [x1, x3, x2]
-        · exact List.Perm.swap x1 x3 [x2]
-        · simp
-          exact List.Perm.swap x2 x3 []
-      · trans [x3, x1, x2]
-        · simp
-          exact List.Perm.swap x1 x2 []
-        · trans [x1, x3, x2]
-          · exact List.Perm.swap x1 x3 [x2]
-          · simp
-            exact List.Perm.swap x2 x3 []
-
-lemma _root_.List.lowPermutations_empty_of_not_le_three :
-    (l : List (ℤ × ℤ)) → (hl : ¬ l.length ≤ 3) → l.lowPermutations = []
-| [], hl => by simp at hl
-| x :: [], hl => by simp at hl
-| x1 :: x2 :: [], hl => by simp at hl
-| x1 :: x2 :: x3 :: [], hl => by simp at hl
-| _ :: _ :: _ :: _ :: _, hl => rfl
 
 namespace FTheory
 
@@ -244,7 +37,7 @@ variable {I : CodimensionOneConfig}
 namespace FiveQuanta
 
 /-- The list of `FiveQuanta` which arise from `charges` and `fluxes`.
-  Note: This gives junk unless `charges` has length less than or equal to `3`,
+  Note: This gives junk unless
   the charges correspond to a `CodimensionOneConfig`
   and `fluxes` has no exotics and no zero entries. -/
 def fromParts (I : CodimensionOneConfig) (charges : Multiset ℤ) (fluxes : FluxesFive) :
@@ -252,24 +45,19 @@ def fromParts (I : CodimensionOneConfig) (charges : Multiset ℤ) (fluxes : Flux
   if charges.card ≠ fluxes.card then {} else
   let chargesList : List ℤ := I.fiveChargeMultisetToList charges
   let fluxesList : List (ℤ × ℤ) := FluxesFive.toList fluxes
-  let fluxesPerms : List (List (ℤ × ℤ)) := fluxesList.lowPermutations
+  let fluxesPerms : List (List (ℤ × ℤ)) := fluxesList.permutations'.dedup
   fluxesPerms.map (fun l => chargesList.zip l)
 
 lemma self_mem_fromParts_of_toCharges_toFluxesFive (I : CodimensionOneConfig) (F : FiveQuanta)
     (hf : F.toFluxesFive.NoExotics ∧ F.toFluxesFive.HasNoZero)
-    (hc : ∀ s ∈ F.toCharges, s ∈ I.allowedBarFiveCharges)
-    (hcard : Multiset.card F ≤ 3) :
+    (hc : ∀ s ∈ F.toCharges, s ∈ I.allowedBarFiveCharges) :
     F ∈ fromParts I F.toCharges F.toFluxesFive := by
   simp [fromParts]
   apply And.intro
   · simp [toCharges, toFluxesFive]
   use (F.toList I).map Prod.snd
   constructor
-  · apply List.lowPermutations_perm_mem_of_length_le_three
-    · exact List.Perm.symm (toList_prod_snd_perm hf hc)
-    · rw [FluxesFive.toList_length F.toFluxesFive hf]
-      simp [toFluxesFive]
-      exact hcard
+  · exact (toList_prod_snd_perm hf hc)
   · rw [← toList_prod_fst_eq hf hc]
     conv_rhs => rw [← coe_toList hf hc]
     congr
@@ -280,21 +68,13 @@ lemma card_eq_charges_card_of_mem_fromParts (I : CodimensionOneConfig) (charges 
     (hc : ∀ s ∈ charges, s ∈ I.allowedBarFiveCharges) :
     ∀ F ∈ fromParts I charges fluxes, F.card = charges.card := by
   intro F hF
-  simp? [fromParts] at hF says
-    simp only [fromParts, ne_eq, List.empty_eq, ite_not, List.mem_ite_nil_right, List.mem_map] at hF
+  simp only [fromParts, ne_eq, List.empty_eq, ite_not, List.mem_ite_nil_right, List.mem_map] at hF
   obtain ⟨hcard, l, hperm, rfl⟩ := hF
   simp only [Multiset.coe_card, List.length_zip]
   rw [CodimensionOneConfig.fiveChargeMultisetToList_length I charges hc]
   rw [hcard]
-  have hflux : fluxes.toList.length ≤ 3 := by
-    by_contra hn
-    rw [List.lowPermutations_empty_of_not_le_three] at hperm
-    simp at hperm
-    exact hn
-  have hl : l.Perm fluxes.toList := by
-    apply List.perm_of_mem_lowPermutations_of_length_le_three
-    · exact hperm
-    · exact hflux
+  rw [List.mem_dedup] at hperm
+  have hl : l.Perm fluxes.toList := List.mem_permutations'.mp hperm
   have hl : l.length = fluxes.toList.length := by
     rw [List.Perm.length_eq hl]
   rw [FluxesFive.toList_length fluxes hf] at hl
@@ -310,46 +90,23 @@ lemma card_eq_fluxes_card_of_mem_fromParts (I : CodimensionOneConfig) (charges :
   simp [fromParts] at hF
   exact hF.1
 
-lemma card_le_three_of_mem_fromPart (I : CodimensionOneConfig) (charges : Multiset ℤ)
-    (fluxes : FluxesFive) (hf : fluxes.NoExotics ∧ fluxes.HasNoZero)
-    (hc : ∀ s ∈ charges, s ∈ I.allowedBarFiveCharges) :
-    ∀ F ∈ fromParts I charges fluxes, F.card ≤ 3 := by
-  intro F hF
-  rw [card_eq_fluxes_card_of_mem_fromParts I charges fluxes hf hc F hF]
-  by_contra hn
-  simp? [fromParts] at hF says
-    simp only [fromParts, ne_eq, List.empty_eq, ite_not, List.mem_ite_nil_right, List.mem_map] at hF
-  obtain ⟨hcard, l, hperm, rfl⟩ := hF
-  rw [List.lowPermutations_empty_of_not_le_three] at hperm
-  simp only [List.not_mem_nil] at hperm
-  rw [FluxesFive.toList_length fluxes hf]
-  exact hn
-
 lemma fromParts_eq_preimage (I : CodimensionOneConfig) (charges : Multiset ℤ) (fluxes : FluxesFive)
     (hf : fluxes.NoExotics ∧ fluxes.HasNoZero)
     (hc : ∀ s ∈ charges, s ∈ I.allowedBarFiveCharges)
     (F : FiveQuanta) :
-    F.toCharges = charges ∧ F.toFluxesFive = fluxes ∧ F.card ≤ 3 ↔
+    F.toCharges = charges ∧ F.toFluxesFive = fluxes ↔
       F ∈ fromParts I charges fluxes := by
   constructor
-  · intro ⟨h1, h2, h3⟩
+  · intro ⟨h1, h2⟩
     subst h1 h2
-    (expose_names; exact self_mem_fromParts_of_toCharges_toFluxesFive I F hf hc h3)
+    exact self_mem_fromParts_of_toCharges_toFluxesFive I F hf hc
   · intro h
-    have F_card := card_le_three_of_mem_fromPart I charges fluxes hf hc F h
-    simp only [F_card, and_true]
-    have fluxes_length : fluxes.toList.length ≤ 3 := by
-      (expose_names; rw [FluxesFive.toList_length fluxes hf])
-      rw [← card_eq_fluxes_card_of_mem_fromParts I charges fluxes hf hc F h]
-      exact F_card
-    simp? [fromParts] at h says
-      simp only [fromParts, ne_eq, List.empty_eq, ite_not, List.mem_ite_nil_right,
+    simp only [fromParts, ne_eq, List.empty_eq, ite_not, List.mem_ite_nil_right,
         List.mem_map] at h
     obtain ⟨hcard, l, hperm, rfl⟩ := h
+    rw [List.mem_dedup] at hperm
     have hlflux : l.Perm fluxes.toList := by
-      apply List.perm_of_mem_lowPermutations_of_length_le_three
-      · exact hperm
-      · exact fluxes_length
+      exact List.mem_permutations'.mp hperm
     have l_length: l.length = charges.card := by
       rw [List.Perm.length_eq hlflux]
       rw [hcard]
@@ -377,25 +134,51 @@ lemma fromParts_eq_preimage (I : CodimensionOneConfig) (charges : Multiset ℤ) 
         refine Multiset.coe_eq_coe.mpr ?_
         exact hlflux
 
-lemma fromParts_eq_preimage_of_charges_card_le_three (I : CodimensionOneConfig)
-    (charges : Multiset ℤ) (fluxes : FluxesFive)
-    (hf : fluxes.NoExotics ∧ fluxes.HasNoZero)
-    (hc : ∀ s ∈ charges, s ∈ I.allowedBarFiveCharges)
-    (F : FiveQuanta) (hcard : charges.card ≤ 3) :
-    F.toCharges = charges ∧ F.toFluxesFive = fluxes ↔ F ∈ fromParts I charges fluxes := by
-  rw [← fromParts_eq_preimage I charges fluxes hf hc F]
-  simp only [and_congr_right_iff, iff_self_and]
-  intro h1 h2
-  have hx : Multiset.card F = charges.card := by
-    rw [← h1]
-    simp [toCharges]
-  rw [hx]
-  exact hcard
-
 /-- The multiset of `FiveQuanta` obtained from a mutliset of charges `Multiset ℤ`,
   which have a `FluxesFive` in `FluxesFive.elemsNoExotics`. -/
 def ofCharges (I : CodimensionOneConfig) (c : Multiset ℤ) : Multiset FiveQuanta :=
   FluxesFive.elemsNoExotics.bind fun f => fromParts I c f
+
+lemma mem_ofCharges_iff (I : CodimensionOneConfig) (charges : Multiset ℤ)
+    (hc : ∀ s ∈ charges, s ∈ I.allowedBarFiveCharges) (F : FiveQuanta) :
+    F ∈ ofCharges I charges ↔
+      F.toCharges = charges ∧ F.toFluxesFive.NoExotics ∧ F.toFluxesFive.HasNoZero := by
+  constructor
+  · intro h
+    simp [ofCharges] at h
+    obtain ⟨f, hf, hF⟩ := h
+    rw [← fromParts_eq_preimage] at hF
+    obtain ⟨h1, h2⟩ := hF
+    subst h1 h2
+    simp only [true_and]
+    constructor
+    · exact FluxesFive.noExotics_of_mem_elemsNoExotics F.toFluxesFive hf
+    · exact FluxesFive.hasNoZero_of_mem_elemsNoExotics F.toFluxesFive hf
+    constructor
+    · exact FluxesFive.noExotics_of_mem_elemsNoExotics f hf
+    · exact FluxesFive.hasNoZero_of_mem_elemsNoExotics f hf
+    · exact hc
+  · intro ⟨rfl, h2, h3⟩
+    simp [ofCharges]
+    use F.toFluxesFive
+    refine ⟨FluxesFive.mem_elemsNoExotics_of_noExotics F.toFluxesFive h2 h3, ?_⟩
+    rw [← fromParts_eq_preimage I F.toCharges F.toFluxesFive]
+    · simp
+    · simp_all
+      exact h3
+    · exact hc
+
+lemma mem_ofCharges_self (I : CodimensionOneConfig) (c : FiveQuanta)
+    (h : c.toFluxesFive.NoExotics) (hnz : c.toFluxesFive.HasNoZero)
+    (hc : ∀ s ∈ c.toCharges, s ∈ I.allowedBarFiveCharges) :
+    c ∈ ofCharges I c.toCharges := by
+  simp [ofCharges]
+  use c.toFluxesFive
+  refine ⟨FluxesFive.mem_elemsNoExotics_of_noExotics c.toFluxesFive h hnz, ?_⟩
+  rw [← fromParts_eq_preimage I c.toCharges c.toFluxesFive]
+  simp only [and_self]
+  exact ⟨h, hnz⟩
+  exact hc
 
 end FiveQuanta
 
@@ -408,7 +191,7 @@ end FiveQuanta
 namespace TenQuanta
 
 /-- The list of `TenQuanta` which arise from `charges` and `fluxes`.
-  Note: This gives junk unless `charges` has length less than or equal to `3`,
+  Note: This gives junk unless `charges`
   the charges correspond to a `CodimensionOneConfig`
   and `fluxes` has no exotics and no zero entries. -/
 def fromParts (I : CodimensionOneConfig) (charges : Multiset ℤ) (fluxes : FluxesTen) :
@@ -416,24 +199,19 @@ def fromParts (I : CodimensionOneConfig) (charges : Multiset ℤ) (fluxes : Flux
   if charges.card ≠ fluxes.card then {} else
   let chargesList : List ℤ := I.tenChargeMultisetToList charges
   let fluxesList : List (ℤ × ℤ) := FluxesTen.toList fluxes
-  let fluxesPerms : List (List (ℤ × ℤ)) := fluxesList.lowPermutations
+  let fluxesPerms : List (List (ℤ × ℤ)) := fluxesList.permutations'.dedup
   fluxesPerms.map (fun l => chargesList.zip l)
 
 lemma self_mem_fromParts_of_toCharges_toFluxesTen (I : CodimensionOneConfig) (F : TenQuanta)
     (hf : F.toFluxesTen.NoExotics ∧ F.toFluxesTen.HasNoZero)
-    (hc : ∀ s ∈ F.toCharges, s ∈ I.allowedTenCharges)
-    (hcard : Multiset.card F ≤ 3) :
+    (hc : ∀ s ∈ F.toCharges, s ∈ I.allowedTenCharges) :
     F ∈ fromParts I F.toCharges F.toFluxesTen := by
   simp [fromParts]
   apply And.intro
   · simp [toCharges, toFluxesTen]
   use (F.toList I).map Prod.snd
   constructor
-  · apply List.lowPermutations_perm_mem_of_length_le_three
-    · exact List.Perm.symm (toList_prod_snd_perm hf hc)
-    · rw [FluxesTen.toList_length F.toFluxesTen hf]
-      simp [toFluxesTen]
-      exact hcard
+  · exact (toList_prod_snd_perm hf hc)
   · rw [← toList_prod_fst_eq hf hc]
     conv_rhs => rw [← coe_toList hf hc]
     congr
@@ -444,21 +222,14 @@ lemma card_eq_charges_card_of_mem_fromParts (I : CodimensionOneConfig) (charges 
     (hc : ∀ s ∈ charges, s ∈ I.allowedTenCharges) :
     ∀ F ∈ fromParts I charges fluxes, F.card = charges.card := by
   intro F hF
-  simp? [fromParts] at hF says
-    simp only [fromParts, ne_eq, List.empty_eq, ite_not, List.mem_ite_nil_right, List.mem_map] at hF
+  simp only [fromParts, ne_eq, List.empty_eq, ite_not, List.mem_ite_nil_right, List.mem_map] at hF
   obtain ⟨hcard, l, hperm, rfl⟩ := hF
   simp only [Multiset.coe_card, List.length_zip]
   rw [CodimensionOneConfig.tenChargeMultisetToList_length I charges hc]
   rw [hcard]
-  have hflux : fluxes.toList.length ≤ 3 := by
-    by_contra hn
-    rw [List.lowPermutations_empty_of_not_le_three] at hperm
-    simp at hperm
-    exact hn
+  rw [List.mem_dedup] at hperm
   have hl : l.Perm fluxes.toList := by
-    apply List.perm_of_mem_lowPermutations_of_length_le_three
-    · exact hperm
-    · exact hflux
+    exact List.mem_permutations'.mp hperm
   have hl : l.length = fluxes.toList.length := by
     rw [List.Perm.length_eq hl]
   rw [FluxesTen.toList_length fluxes hf] at hl
@@ -474,42 +245,20 @@ lemma card_eq_fluxes_card_of_mem_fromParts (I : CodimensionOneConfig) (charges :
   simp [fromParts] at hF
   exact hF.1
 
-lemma card_le_three_of_mem_fromPart (I : CodimensionOneConfig) (charges : Multiset ℤ)
-    (fluxes : FluxesTen) (hf : fluxes.NoExotics ∧ fluxes.HasNoZero)
-    (hc : ∀ s ∈ charges, s ∈ I.allowedTenCharges) :
-    ∀ F ∈ fromParts I charges fluxes, F.card ≤ 3 := by
-  intro F hF
-  rw [card_eq_fluxes_card_of_mem_fromParts I charges fluxes hf hc F hF]
-  by_contra hn
-  simp [fromParts] at hF
-  obtain ⟨hcard, l, hperm, rfl⟩ := hF
-  rw [List.lowPermutations_empty_of_not_le_three] at hperm
-  simp at hperm
-  rw [FluxesTen.toList_length fluxes hf]
-  exact hn
-
 lemma fromParts_eq_preimage (I : CodimensionOneConfig) (charges : Multiset ℤ) (fluxes : FluxesTen)
     (hf : fluxes.NoExotics ∧ fluxes.HasNoZero)
     (hc : ∀ s ∈ charges, s ∈ I.allowedTenCharges) (F : TenQuanta) :
-    F.toCharges = charges ∧ F.toFluxesTen = fluxes ∧ F.card ≤ 3 ↔
+    F.toCharges = charges ∧ F.toFluxesTen = fluxes ↔
       F ∈ fromParts I charges fluxes := by
   constructor
-  · intro ⟨h1, h2, h3⟩
+  · intro ⟨h1, h2⟩
     subst h1 h2
-    (expose_names; exact self_mem_fromParts_of_toCharges_toFluxesTen I F hf hc h3)
+    exact self_mem_fromParts_of_toCharges_toFluxesTen I F hf hc
   · intro h
-    have F_card := card_le_three_of_mem_fromPart I charges fluxes hf hc F h
-    simp only [F_card, and_true]
-    have fluxes_length : fluxes.toList.length ≤ 3 := by
-      (expose_names; rw [FluxesTen.toList_length fluxes hf])
-      rw [← card_eq_fluxes_card_of_mem_fromParts I charges fluxes hf hc F h]
-      exact F_card
     simp [fromParts] at h
     obtain ⟨hcard, l, hperm, rfl⟩ := h
     have hlflux : l.Perm fluxes.toList := by
-      apply List.perm_of_mem_lowPermutations_of_length_le_three
-      · exact hperm
-      · exact fluxes_length
+      exact hperm
     have l_length: l.length = charges.card := by
       rw [List.Perm.length_eq hlflux]
       rw [hcard]
@@ -537,27 +286,64 @@ lemma fromParts_eq_preimage (I : CodimensionOneConfig) (charges : Multiset ℤ) 
         refine Multiset.coe_eq_coe.mpr ?_
         exact hlflux
 
-lemma fromParts_eq_preimage_of_charges_card_le_three (I : CodimensionOneConfig)
-    (charges : Multiset ℤ) (fluxes : FluxesTen)
-    (hf : fluxes.NoExotics ∧ fluxes.HasNoZero)
-    (hc : ∀ s ∈ charges, s ∈ I.allowedTenCharges)
-    (F : TenQuanta) (hcard : charges.card ≤ 3) :
-    F.toCharges = charges ∧ F.toFluxesTen = fluxes ↔ F ∈ fromParts I charges fluxes := by
-  rw [← fromParts_eq_preimage I charges fluxes hf hc F]
-  simp only [and_congr_right_iff, iff_self_and]
-  intro h1 h2
-  have hx : Multiset.card F = charges.card := by
-    rw [← h1]
-    simp [toCharges]
-  rw [hx]
-  exact hcard
-
 /-- The multiset of `TenQuanta` obtained from a mutliset of charges `Multiset ℤ`,
   which have a `FluxesTen` in `FluxesTen.elemsNoExotics`. -/
-def ofCharges (I : CodimensionOneConfig) (c : Multiset ℤ) : Multiset FiveQuanta :=
+def ofCharges (I : CodimensionOneConfig) (c : Multiset ℤ) : Multiset TenQuanta :=
   FluxesTen.elemsNoExotics.bind fun f => fromParts I c f
 
+lemma mem_ofCharges_iff (I : CodimensionOneConfig) (charges : Multiset ℤ)
+    (hc : ∀ s ∈ charges, s ∈ I.allowedTenCharges) (F : TenQuanta) :
+    F ∈ ofCharges I charges ↔
+      F.toCharges = charges ∧ F.toFluxesTen.NoExotics ∧ F.toFluxesTen.HasNoZero := by
+  constructor
+  · intro h
+    simp [ofCharges] at h
+    obtain ⟨f, hf, hF⟩ := h
+    rw [← fromParts_eq_preimage] at hF
+    obtain ⟨h1, h2⟩ := hF
+    subst h1 h2
+    simp only [true_and]
+    constructor
+    · exact FluxesTen.noExotics_of_mem_elemsNoExotics F.toFluxesTen hf
+    · exact FluxesTen.hasNoZero_of_mem_elemsNoExotics F.toFluxesTen hf
+    constructor
+    · exact FluxesTen.noExotics_of_mem_elemsNoExotics f hf
+    · exact FluxesTen.hasNoZero_of_mem_elemsNoExotics f hf
+    · exact hc
+  · intro ⟨rfl, h2, h3⟩
+    simp [ofCharges]
+    use F.toFluxesTen
+    refine ⟨FluxesTen.mem_elemsNoExotics_of_noExotics F.toFluxesTen h2 h3, ?_⟩
+    rw [← fromParts_eq_preimage I F.toCharges F.toFluxesTen]
+    · simp
+    · simp_all
+      exact h3
+    · exact hc
+
+lemma mem_ofCharges_self (I : CodimensionOneConfig) (c : TenQuanta)
+    (h : c.toFluxesTen.NoExotics) (hnz : c.toFluxesTen.HasNoZero)
+    (hc : ∀ s ∈ c.toCharges, s ∈ I.allowedTenCharges) :
+    c ∈ ofCharges I c.toCharges := by
+  simp [ofCharges]
+  use c.toFluxesTen
+  refine ⟨FluxesTen.mem_elemsNoExotics_of_noExotics c.toFluxesTen h hnz, ?_⟩
+  rw [← fromParts_eq_preimage I c.toCharges c.toFluxesTen]
+  simp only [and_self]
+  exact ⟨h, hnz⟩
+  exact hc
+
 end TenQuanta
+
+namespace Quanta
+
+/-- The multiset of `Quanta` obtained from a `Charges`,
+  which have a `Fluxes` which do not permit exotics. -/
+def ofCharges (I : CodimensionOneConfig) (c : Charges) : Multiset Quanta :=
+    let c1 := FiveQuanta.ofCharges I c.2.2.1.val
+    let c2 := TenQuanta.ofCharges I c.2.2.2.val
+    (c1.product c2).map fun (F, T) => (c.1, c.2.1, F, T)
+
+end Quanta
 
 end SU5U1
 
