PhysLean/StringTheory/FTheory/SU5U1/Fluxes/NoExotics/ToList.lean
@@ -4,7 +4,6 @@ Released under Apache 2.0 license as described in the file LICENSE.
 Authors: Joseph Tooby-Smith
 -/
 import PhysLean.StringTheory.FTheory.SU5U1.Fluxes.NoExotics.Completeness
-import PhysLean.StringTheory.FTheory.SU5U1.Charges.Tree.Basic
 /-!
 
 # Fluxes into list
